

(Q1) Consider the group $(\mathbb{Z}/p\mathbb{Z})^\times$. The only subgroups of $(\mathbb{Z}/p\mathbb{Z})^\times$ have an order of that divides $p-1$ (the order of the group $(\mathbb{Z}/p\mathbb{Z})^\times$).

Note that since $p \nmid a$, it is congruent mod p to some element $b \in (\mathbb{Z}/p\mathbb{Z})^\times$.

$$a \equiv b \pmod{p}.$$

Now the order of b must divide $p-1$. Let o be the order of b :

$$b^o \equiv 1 \pmod{p}.$$

Since $0 \mid p-1 \Rightarrow \exists m \in \mathbb{Z}^+ : 0m = p-1$

$$b^0 \equiv 1 \pmod{p}$$

$$(b^0)^m = (1)^m \pmod{p}$$

$$b^{p-1} \equiv 1 \pmod{p}$$

Thus, $a^{p-1} \equiv 1 \pmod{p}$

(Q3) To show that H is a normal subgroup, we have to show that for any $g \in G$ and $h \in H$, $(ghg^{-1}) \in H$.

$$\begin{aligned} ghg^{-1} &= gg^{-1}h \quad (\text{since } G \text{ is abelian}) \\ &= e_{G_2} h = h \end{aligned}$$

$h \in H$ (by assumption). Thus, $H \trianglelefteq G$ for any subgroup of an abelian group.

Note: Equivalent definitions of normal subgroups.

- (i) For every $g \in G$, we have that $gN = Ng$.
- (ii) For every $g \in G$ and $n \in N$, $gng^{-1} \in N$.

i \rightarrow ii Since $gN = Ng$, every element of gN is also an element Ng . For all $g \in G$ and $n \in N$, we can find an $n' \in N$ such that $gn = n'g$. Thus, $gn \cdot g^{-1} = n' \cdot g \cdot (g^{-1}) \Rightarrow gng^{-1} = n'$. Since $n' \in N$, $gng^{-1} \in N$.

ii \rightarrow i For every $g \in G$ and $n \in N$, $gng^{-1} = n'$ for some $n' \in N$. Thus, $gng^{-1} \cdot (g) = n' \cdot g \Rightarrow gn = n'g$ and finally $gN = Ng$.

A ^{sub}group H in G_1 is said to be normal if for all $h \in H$ and $g \in G_1$, we have that $(ghg^{-1}) \in H$.

(Q5) Consider a homomorphism $\varphi : G_1 \rightarrow G_2$. We have to show $\text{Ker}(\varphi) \trianglelefteq G_1$ is a normal subgroup of G_1 .

Let $x \in G_1$ and $k \in \text{Ker}(\varphi)$. Now consider $\varphi(x \cdot k \cdot x^{-1})$.

$$\begin{aligned}\varphi(x \cdot k \cdot x^{-1}) &= \varphi(x) \cdot \varphi(k) \cdot \varphi(x^{-1}) \\ &= \varphi(x) \cdot e_{G_2} \cdot [\varphi(x)]^{-1} \\ &= \varphi(x) \cdot [\varphi(x)]^{-1} \\ &= e_{G_2}.\end{aligned}$$

Thus, $xkx^{-1} \in \text{Ker}(\varphi)$, and $\text{Ker}(\varphi) \trianglelefteq G_1$.

(Q7)

- If a subgroup $K \leq G_1$ is normal in G_1 , then there exists a homomorphism $\varphi: G_1 \rightarrow H$ such that $K = \ker(\varphi)$.
- Consider the function $\varphi: G_1 \rightarrow G_1/K$ (Since K is normal G_1/K is a well-defined group), such that $\varphi(g) = gK$.

$$\begin{aligned}\text{First, } \varphi(g_1 \cdot g_2) &= (g_1 \cdot g_2)K = (g_1K) \oplus (g_2K) \\ &= \varphi(g_1) \oplus \varphi(g_2)\end{aligned}$$

Thus φ is a homomorphism.

- $\ker(\varphi) = ?$.

$$\begin{aligned}\varphi(g) = eK &\Rightarrow gK = eK \Rightarrow (e^{-1})(g) \in K \\ &\Rightarrow g \in K.\end{aligned}$$

Thus, $K = \ker(\varphi)$

- The backward direction is as a result of Problem 5 (the kernel is a normal subgroup).

(Q8) Part I:

- First, we prove that $Z(G)$ is a subgroup of G .

$$Z(G) = [z \in G : zg = gz, \forall g \in G]$$

1. Now, $e \in Z(G)$ since $e \cdot g = g = g \cdot e$

2. Given $g_1 \in Z(G) \Rightarrow g_1 g = g g_1 \quad \forall g \in G$
and $g_2 \in Z(G) \Rightarrow g_2 g' = g' g_2 \quad \forall g' \in G$

$$\begin{aligned} \cdot \quad g_1 g &= g g_1 \Rightarrow g = g_1^{-1} g g_1 \\ \cdot \quad g_2 g &= g g_2 \Rightarrow \end{aligned} \quad \left. \vphantom{\begin{aligned} \cdot \quad g_1 g &= g g_1 \\ \cdot \quad g_2 g &= g g_2 \end{aligned}} \right\} \text{OMIT}$$

$$\begin{aligned} (g_1 \cdot g_2) \cdot x &= g_1 \cdot (g_2 \cdot x) = g_1 \cdot (x \cdot g_2) \\ &= (g_1 \cdot x) \cdot g_2 \\ &= (x \cdot g_1) \cdot g_2 \end{aligned}$$

$$\begin{aligned} \text{Thus, } (g_1 \cdot g_2) \cdot x &= x \cdot (g_1 \cdot g_2) \\ &= x \cdot g_1 \cdot g_2 \end{aligned}$$

3. Given $g \in Z(G) \Rightarrow g g' = g' g \quad \forall g' \in G$
Now,

- Now we show that $Z(G_1)$ is a normal subgroup.
- That is, for any $g \in G_1$ and $z \in Z(G_1)$ we have to show that $g \cdot z \cdot g^{-1} \in Z(G_1)$

$$\begin{aligned} g \cdot z \cdot g^{-1} &= g \cdot (z \cdot g^{-1}) = g \cdot (g^{-1} \cdot z) \\ &= (g \cdot g^{-1}) \cdot z = e \cdot z = z \in Z(G_1). \end{aligned}$$

Thus $Z(G_1) \trianglelefteq G_1$.

• Part II :

If $G_1/Z(G_1)$ is cyclic, then there exists $x \in G_1$ such that $G_1/Z(G_1) = \langle xZ(G_1) \rangle$. Thus for any $g \in G_1$, there exists $m \in \mathbb{Z}$ such that $gZ(G_1) = x^m Z(G_1) \Rightarrow (x^m)^{-1}(g) \in Z(G_1)$
 $(x^{-m})(g) \in Z(G_1) \Rightarrow \forall n \in G_1$, we have:
 $(x^{-m})(g)(n) = (n)(g)(x^{-m})$.

Now, let $g = (x^m)(a) = (a)(x^m)$ Substitute $n = e$ in the above equation.

$$\begin{aligned} (x^{-m})(x^m)(a)(n) &= (n)(a)(x^m)(x^{-m}) \\ (a)(n) &= (n)(a) \Rightarrow G_1 \text{ is abelian.} \end{aligned}$$

(Q10) In our proof, we use the following result: In a group G_1 , if $|G_1| = p^n$ where p is a prime and $n \in \mathbb{Z}^+$, then the centre of G_1 is nontrivial.

Proof.

- Since $|G| = p^2$, and $Z(G)$ is nontrivial, we have two options:

1. $|Z(G)| = p^2$. But since $|G| = p^2$,

$Z(G) = G \Rightarrow G$ is abelian.

2. $|Z(G)| = p$. Thus, by Lagrange's theorem,

$[G : Z(G)] = |G \setminus Z(G)| = p$. Since the order of the group $G \setminus Z(G)$ is cyclic.

Thus, by applying the theorem proved in (Q8), we get G is abelian.

(Q9) Lemma 3.1 may be rephrased as:

Let G be a group and H be a subgroup of G . If aH and bH are two cosets of H in G , and if $(aH) \cap (bH) \neq \emptyset$, then we have that $aH = bH$.

If $(aH) \cap (bH) \neq \emptyset$, then there exists at least one $s \in (aH)$ and $s \in (bH)$.

Since $s \in (aH)$, $aH = sH$. Similarly, since $s \in (bH)$, $bH = sH$. Thus, $aH = sH = bH$ and $aH = bH$.

Q.E.D.

The above proof uses the following lemma:

Let G be a group and H be a subgroup of G . For any $a' \in aH$ ($a \in G$), we have that $a'H = aH$.

Proof: Since $a' \in aH$, there exists $h' \in H$ such that $a' = ah'$. $aH = [ah : h \in H]$ and $a'H = [a'h : h \in H] = [(ah')(h) : h \in H] = [a(h'h) : h \in H] = [ag : g \in H]$. Note that $(h'h) \in H$ since H is a subgroup and is closed under multiplication.

Note: $|aH| = |H| = |a'H|$ for any $a \in G$ and $a' \in G$.

Define a function $\varphi: H \rightarrow aH$ ($a \in G$),
such that $\varphi(h) = ah$. We will show
 φ is a bijection.

- $\varphi(h_2) = \varphi(h_1)$
 $\Rightarrow ah_2 = ah_1$
 $\Rightarrow a^{-1}(ah_2) = a^{-1}(ah_1)$
 $\Rightarrow (a^{-1}a)h_2 = (a^{-1}a)h_1$
 $\Rightarrow eh_2 = eh_1$
 $\Rightarrow h_2 = h_1$.

Thus φ is injective.

- Given any $\alpha \in aH$ such that, $\alpha = ah'$
for a $h' \in H$. Note that $h' \in H$ is
such that $\varphi(h') = \alpha = ah'$. Thus φ is
surjective.

Since there exists a bijection between
the sets H and aH , they must be
of the same size.